Add IR for bitfid

SSA/Experimental/Bits/IR.lean
@@ -1,4 +1,5 @@
 import SSA.Core.WellTypedFramework
+import SSA.Core.Util
 import SSA.Experimental.Bits.Decide
 
 inductive BaseType
@@ -7,16 +8,79 @@ inductive BaseType
 
 instance : Inhabited BaseType := ⟨BaseType.bitvec⟩
 
+def Term.equiv : Term → Term → Prop
+  | t₁, t₂ => t₁.eval = t₂.eval
+
+def Term.equiv_refl : ∀ t, Term.equiv t t := by
+  intro t
+  simp [Term.equiv, Term.eval]
+
+def Term.equiv_symm {t₁ t₂ : Term} : Term.equiv t₁ t₂ → Term.equiv t₂ t₁ := by
+  intro h
+  simp [Term.equiv, Term.eval] at *
+  rw [h]
+
+def Term.equiv_trans {t₁ t₂ t₃ : Term} : Term.equiv t₁ t₂ → Term.equiv t₂ t₃ → Term.equiv t₁ t₃ := by
+  intro h₁ h₂
+  simp [Term.equiv, Term.eval] at *
+  rw [h₁, h₂]
+
+def Term.equiv_equiv : Equivalence Term.equiv := ⟨Term.equiv_refl, Term.equiv_symm, Term.equiv_trans⟩
+
+instance instSetoid : Setoid Term := ⟨Term.equiv, Term.equiv_equiv⟩
+
+def Bitvec := Quotient instSetoid
+
+def Term.equiv_pair : Term × Term → Term × Term → Prop
+  | (t₁, t₂), (t₁',t₂') => Term.equiv t₁ t₁' ∧ Term.equiv t₂ t₂'
+
+namespace Bitvec
+
+theorem and_equiv : ∀ {x y x' y' : Term}, 
+  x ≈ x' → y ≈ y' → (Term.and x y) ≈ (Term.and x' y') := by
+  {
+    intro x y x' y' hx hy
+    simp [HasEquiv.Equiv, Setoid.r, Term.equiv, Term.and, Term.eval]
+    rw [hx, hy]
+  }
+
+  theorem and_equiv_lift₁ : ∀ (a b₁ b₂ : Term), b₁ ≈ b₂ → 
+  Quotient.mk instSetoid (Term.and a b₁) = Quotient.mk instSetoid (Term.and a b₂) := by
+  intro _ _ _ h
+  simp [HasEquiv.Equiv, Setoid.r, Term.equiv, Term.and, Term.eval]
+  rw [h]
+
+  theorem and_equiv_lift₂ : ∀ (a₁ a₂ b : Term), a₁ ≈ a₂ → 
+  Quotient.mk instSetoid (Term.and a₁ b) = Quotient.mk instSetoid (Term.and a₂ b) := by
+  intro _ _ _ h
+  simp [HasEquiv.Equiv, Setoid.r, Term.equiv, Term.and, Term.eval]
+  rw [h]
+
+def and : Bitvec → Bitvec → Bitvec := Quot.lift₂ (fun t₁ t₂ => Quotient.mk instSetoid $ Term.and t₁ t₂) and_equiv_lift₁ and_equiv_lift₂
+
+theorem not_equiv {x x' : Term} : x ≈ x' → (Term.not x) ≈ (Term.not x') := by
+  intro hx
+  simp [HasEquiv.Equiv, Setoid.r, Term.equiv, Term.not, Term.eval]
+  rw [hx]
+
+-- These should be automatically generated somehow
+theorem not_equiv_lift {x x' : Term} : x ≈ x' → 
+  Quotient.mk instSetoid (Term.not x) = Quotient.mk instSetoid (Term.not x') := by
+  intro hx
+  simp [HasEquiv.Equiv, Setoid.r, Term.equiv, Term.not, Term.eval]
+  rw [hx]
+
+def not : Bitvec → Bitvec := Quotient.lift (fun t => Quotient.mk instSetoid $ Term.not t) @not_equiv_lift
+
+end Bitvec
+
 instance : Goedel BaseType where
 toType := fun
-  | .bitvec => Term
+  | .bitvec => Bitvec
 
 abbrev UserType := SSA.UserType BaseType
 
 inductive Op : Type
-| zero
-| negOne
-| one
 | and
 | or
 | xor
@@ -27,13 +91,14 @@ inductive Op : Type
 | neg
 | incr
 | decr
+| const : Term → Op
 
 @[simp, reducible]
 def argUserType : Op → UserType
-| Op.zero  | Op.negOne | Op.one => .unit
 | Op.and | Op.or | Op.xor | Op.add | Op.sub => 
   .pair (.base (BaseType.bitvec)) (.base (BaseType.bitvec))
 | Op.not | Op.ls | Op.neg | Op.incr | Op.decr => .base (BaseType.bitvec)
+| Op.const _ => .unit
 
 @[simp, reducible]
 def outUserType : Op → UserType := fun _ => .base BaseType.bitvec
@@ -50,19 +115,18 @@ def eval (o : Op)
   (_rgn : (Goedel.toType (rgnDom o) → Goedel.toType (rgnCod o))) :
   Goedel.toType (outUserType o) :=
     match o with
-     | Op.zero => Term.zero
-     | Op.negOne => Term.negOne
-     | Op.one => Term.one
-     | Op.and => Term.and arg.1 arg.2
-     | Op.or => Term.or arg.1 arg.2
-     | Op.xor => Term.xor arg.1 arg.2
-     | Op.not => Term.not arg
-     | Op.ls => Term.ls arg
-     | Op.add => Term.add arg.1 arg.2
-     | Op.sub => Term.sub arg.1 arg.2
-     | Op.neg => Term.neg arg
-     | Op.incr => Term.incr arg
-     | Op.decr => Term.decr arg
+     | Op.and => Bitvec.and arg.1 arg.2
+     | Op.not => Bitvec.not arg
+     | _ => sorry
+     -- | Op.or => Term.or arg.1 arg.2
+     -- | Op.xor => Term.xor arg.1 arg.2
+     -- | Op.ls => Term.ls arg
+     -- | Op.add => Term.add arg.1 arg.2
+     -- | Op.sub => Term.sub arg.1 arg.2
+     -- | Op.neg => Term.neg arg
+     -- | Op.incr => Term.incr arg
+     -- | Op.decr => Term.decr arg
+     -- | Op.const c => c
 
 instance TUS : SSA.TypedUserSemantics Op BaseType where
   argUserType := argUserType
@@ -73,9 +137,6 @@ instance TUS : SSA.TypedUserSemantics Op BaseType where
 
 
 open EDSL
-syntax "zero" term : dsl_op
-syntax "negOne" term : dsl_op
-syntax "one" term : dsl_op
 syntax "and" term : dsl_op
 syntax "or" term : dsl_op
 syntax "xor" term : dsl_op
@@ -86,6 +147,7 @@ syntax "sub" term : dsl_op
 syntax "neg" term : dsl_op
 syntax "incr" term : dsl_op
 syntax "decr" term : dsl_op
+syntax "const" term : dsl_op
 
 macro_rules
   | `([dsl_op| add $w ]) => `(Op.add $w)
@@ -94,11 +156,8 @@ macro_rules
   | `([dsl_op| incr $w ]) => `(Op.incr $w)
   | `([dsl_op| ls $w ]) => `(Op.ls $w)
   | `([dsl_op| neg $w ]) => `(Op.neg $w)
-  | `([dsl_op| negOne $w ]) => `(Op.negOne $w)
-  | `([dsl_op| not $w ]) => `(Op.not $w)
-  | `([dsl_op| one $w ]) => `(Op.one $w)
+  | `([dsl_op| const $w ]) => `($w)
   | `([dsl_op| or $w ]) => `(Op.or $w)
   | `([dsl_op| sub $w ]) => `(Op.sub $w)
   | `([dsl_op| xor $w ]) => `(Op.xor $w)
-  | `([dsl_op| zero $w ]) => `(Op.zero $w)
 
