SSA/Experimental/Bits/Examples.lean
@@ -1,0 +1,7 @@
+import SSA.Experimental.Bits.Decide
+import SSA.Experimental.Bits.IR
+
+open EDSL in
+
+set_option maxHeartbeats 2000000 in
+example : (Term.not (Term.not (Term.var 1))).eval = (Term.var 1).eval := by decide
